% !TEX spellcheck=en_US
\documentclass[a4paper]{article}
\usepackage[american]{babel}
\usepackage[T1]{fontenc}
\usepackage[utf8]{inputenc}
\usepackage[activate={true,nocompatibility},final,tracking=true,kerning=true,spacing=true,factor=1100,stretch=10,shrink=10]{microtype}
\usepackage{amsmath}
\usepackage{amsthm}
\usepackage{amssymb}
\usepackage{mathtools}
\usepackage{mathmacros/mathmacros}
 
\newtheorem{lemma}{Lemma}
\newtheorem{thm}{Theorem}
\newtheorem{crl}{Corollary}
\newtheorem{definition}{Definition}
\theoremstyle{remark}
\newtheorem{exm}{Example}
\theoremstyle{remark}
\newtheorem{rem}{Remark}

% misc macros
\newcommand*{\pref}[2]{#1 (\ref{#2})}

% microtype
\SetTracking{encoding={*}, shape=sc}{0}
 
\begin{document}
 
\title{Homework Template}
\author{Mazawa Shinonome \\ MATH 101}
 
\maketitle
 
\begin{thm}\label{my-theorem}
Delete this text and write theorem statement here.
\end{thm}
 
\begin{proof}
Blah, blah, blah.  Here is an example of the \texttt{align} environment:
\begin{align*}
    \sum_{i=1}^{k+1}i & = \left(\sum_{i=1}^{k}i\right) +(k+1)                     \\ 
                      & = \frac{k(k+1)}{2}+k+1 & (\text{by inductive hypothesis}) \\
                      & = \frac{k(k+1)+2(k+1)}{2}                                 \\
                      & = \frac{(k+1)(k+2)}{2}                                    \\
                      & = \frac{(k+1)((k+1)+1)}{2}.
\end{align*}
\end{proof}
 
\begin{lemma}
Let $n\in \mathbb{N}$. Using \pref{theorem}{my-theorem} \dots
\end{lemma}
 
\begin{proof}[Disproof]
Blah, blah, blah.

\begin{equation}\label{gradient-operator}
    \fgrad \defines \ihat\frac{\partial}{\partial x} + \jhat\frac{\partial}{\partial y} + \khat\frac{\partial}{\partial z}
\end{equation}

\end{proof}
 
\end{document}
